src/impl/system.lean
@@ -5,54 +5,6 @@ namespace Concrete
 
 open Protocol (Request Response)
 
-def _root_.Protocol.Request.origin? : Request → Option String
-  | .promiseGet req =>
-      some req.id.origin
-  | .promiseCreate req =>
-      some req.id.origin
-  | .promiseSettle req =>
-      some req.id.origin
-  | .promiseRegisterCallback req =>
-      some req.awaited.origin
-  | .promiseRegisterListener req =>
-      some req.awaited.origin
-  | .promiseSearch _ =>
-      none
-  | .scheduleGet _ =>
-      none
-  | .scheduleCreate _ =>
-      none
-  | .scheduleDelete _ =>
-      none
-  | .scheduleSearch _ =>
-      none
-  | .taskGet req =>
-      some req.id.origin
-  | .taskCreate req =>
-      some req.action.id.origin
-  | .taskAcquire req =>
-      some req.id.origin
-  | .taskFence req =>
-      some req.id.origin
-  | .taskHeartbeat req =>
-      match req.tasks with
-      | [] =>
-          none
-      | t :: ts =>
-          if ts.all (·.id.origin == t.id.origin) then some t.id.origin else none
-  | .taskSuspend req =>
-      some req.id.origin
-  | .taskFulfill req =>
-      some req.id.origin
-  | .taskRelease req =>
-      some req.id.origin
-  | .taskHalt req =>
-      some req.id.origin
-  | .taskContinue req =>
-      some req.id.origin
-  | .taskSearch _ =>
-      none
-
 inductive Event
   | external (req : Request)
   | internal (timer : Timer)
@@ -65,75 +17,77 @@ inductive Reply
   | stutter
   deriving Repr, BEq
 
-def handleExternal (now : Nat) (org : Origin) : Request → Response × Commands
+def handleExternal (req : Request) (now : Nat) (org : Origin) : Response × Commands :=
+  match req with
   | .promiseGet req =>
-      let (res, c) := promiseGet now org req
+      let (res, c) := promiseGet req now org
       (.promiseGet res, c)
   | .promiseCreate req =>
-      let (res, c) := promiseCreate now org req
+      let (res, c) := promiseCreate req now org
       (.promiseCreate res, c)
   | .promiseSettle req =>
-      let (res, c) := promiseSettle now org req
+      let (res, c) := promiseSettle req now org
       (.promiseSettle res, c)
   | .promiseRegisterCallback req =>
-      let (res, c) := promiseRegisterCallback now org req
+      let (res, c) := promiseRegisterCallback req now org
       (.promiseRegisterCallback res, c)
   | .promiseRegisterListener req =>
-      let (res, c) := promiseRegisterListener now org req
+      let (res, c) := promiseRegisterListener req now org
       (.promiseRegisterListener res, c)
   | .promiseSearch req =>
-      let (res, c) := promiseSearch now org req
+      let (res, c) := promiseSearch req now org
       (.promiseSearch res, c)
   | .scheduleGet req =>
-      let (res, c) := scheduleGet now org req
+      let (res, c) := scheduleGet req now org
       (.scheduleGet res, c)
   | .scheduleCreate req =>
-      let (res, c) := scheduleCreate now org req
+      let (res, c) := scheduleCreate req now org
       (.scheduleCreate res, c)
   | .scheduleDelete req =>
-      let (res, c) := scheduleDelete now org req
+      let (res, c) := scheduleDelete req now org
       (.scheduleDelete res, c)
   | .scheduleSearch req =>
-      let (res, c) := scheduleSearch now org req
+      let (res, c) := scheduleSearch req now org
       (.scheduleSearch res, c)
   | .taskGet req =>
-      let (res, c) := taskGet now org req
+      let (res, c) := taskGet req now org
       (.taskGet res, c)
   | .taskCreate req =>
-      let (res, c) := taskCreate now org req
+      let (res, c) := taskCreate req now org
       (.taskCreate res, c)
   | .taskAcquire req =>
-      let (res, c) := taskAcquire now org req
+      let (res, c) := taskAcquire req now org
       (.taskAcquire res, c)
   | .taskFence req =>
-      let (res, c) := taskFence now org req
+      let (res, c) := taskFence req now org
       (.taskFence res, c)
   | .taskHeartbeat req =>
-      let (res, c) := taskHeartbeat now org req
+      let (res, c) := taskHeartbeat req now org
       (.taskHeartbeat res, c)
   | .taskSuspend req =>
-      let (res, c) := taskSuspend now org req
+      let (res, c) := taskSuspend req now org
       (.taskSuspend res, c)
   | .taskFulfill req =>
-      let (res, c) := taskFulfill now org req
+      let (res, c) := taskFulfill req now org
       (.taskFulfill res, c)
   | .taskRelease req =>
-      let (res, c) := taskRelease now org req
+      let (res, c) := taskRelease req now org
       (.taskRelease res, c)
   | .taskHalt req =>
-      let (res, c) := taskHalt now org req
+      let (res, c) := taskHalt req now org
       (.taskHalt res, c)
   | .taskContinue req =>
-      let (res, c) := taskContinue now org req
+      let (res, c) := taskContinue req now org
       (.taskContinue res, c)
   | .taskSearch req =>
-      let (res, c) := taskSearch now org req
+      let (res, c) := taskSearch req now org
       (.taskSearch res, c)
 
-def handle (now : Nat) (org : Origin) : Event → Reply × Commands
+def handle (ev : Event) (now : Nat) (org : Origin) : Reply × Commands :=
+  match ev with
   | .external req =>
       let swept := sweep now org
-      let (res, c) := handleExternal now swept.org req
+      let (res, c) := handleExternal req now swept.org
       (.external res, swept.merge c)
   | .internal _ =>
       (.internal, sweep now org)
@@ -145,13 +99,13 @@ def step (H : Hasher) (ev : Event) (now : Nat) (s : State) : Reply × State :=
   | .external req =>
       match req.origin? with
       | some name =>
-          let (r, s', ok) := run H name (fun org => handle now org ev) s
+          let (r, s', ok) := run H name (fun org => handle ev now org) s
           (if ok then r else .stutter, s')
       | none =>
           (.stutter, s)
   | .internal t =>
       if (s.blob? (.timer t)).isSome ∧ t.deadline ≤ now then
-        let (r, s', ok) := run H t.id.origin (fun org => handle now org ev) s
+        let (r, s', ok) := run H t.id.origin (fun org => handle ev now org) s
         (if ok then r else .stutter, s')
       else
         (.stutter, s)
